lean/Hourglass.lean
@@ -2,4 +2,5 @@ import Hourglass.Funs
 import Hourglass.FunsExternal
 import Hourglass.Laws
 import Hourglass.Merge
+import Hourglass.World
 import Hourglass.Trust
